flake.nix
@@ -1,17 +1,7 @@
 {
   inputs = {
-    nix-vscode-extensions.url = "github:nix-community/nix-vscode-extensions";
-    vscoq.url = "github:coq-community/vscoq";
-    flake-utils.follows = "nix-vscode-extensions/flake-utils";
-    nixpkgs.follows = "nix-vscode-extensions/nixpkgs";
-    coq-8_18 = {
-      type = "github";
-      owner = "coq";
-      repo = "coq";
-      ref = "V8.18.0";
-    };
-
-    coq-8_18.inputs.nixpkgs.follows = "nixpkgs";
+    flake-utils.url = "github:numtide/flake-utils";
+    nixpkgs.url = "github:nixos/nixpkgs/nixpkgs-unstable";
   };
 
   outputs = inputs:
@@ -19,32 +9,17 @@
       (system:
         let
           pkgs = inputs.nixpkgs.legacyPackages.${system};
-          extensions = inputs.nix-vscode-extensions.extensions.${system};
-          inherit (pkgs) vscode-with-extensions vscodium;
-
-          packages.default =
-            vscode-with-extensions.override {
-              vscode = vscodium;
-              vscodeExtensions = [
-                extensions.vscode-marketplace.maximedenes.vscoq
-              ];
-            };
 
           devShells.default = pkgs.mkShell {
             buildInputs = [
-              packages.default
-              inputs.coq-8_18.defaultPackage.${system}
-              inputs.vscoq.packages.${system}.vscoq-language-server
-              (inputs.nixpkgs.legacyPackages.${system}.coqPackages.callPackage ./stdpp.nix {})
+              pkgs.coq
+              pkgs.coqPackages.stdpp
+              pkgs.coqPackages.coqide
             ];
-            shellHook = ''
-              printf "VSCodium with extensions:\n"
-              codium --list-extensions
-            '';
           };
         in
         {
-          inherit packages devShells;
+          inherit devShells;
         });
 }
 
